TEST_Strictly_Positiveness_in_AML.v
@@ -1,0 +1,22 @@
+Require Import String.
+Require Import AML_definition.
+
+Definition simple_neg := (sp_not (set "X")).
+Definition X_i_X_i_nX := (sp_impl (set "X") ((sp_impl (set "X") (sp_not (set "X"))))).
+Definition X_imp_X := (sp_impl (set "X") (set "X")).
+Definition X_i_X_i_X := (sp_impl (set "X") ((sp_impl (set "X") (set "X")))).
+
+Lemma test1: (strictly_positive simple_neg (svar_c "X") = false).
+Proof. reflexivity. Qed.
+Lemma test2: (strictly_positive X_imp_X (svar_c "X") = false).
+Proof. reflexivity. Qed.
+Lemma test3: (strictly_positive (sp_not X_imp_X) (svar_c "X") = false).
+Proof. reflexivity. Qed.
+Lemma test4: (strictly_positive X_i_X_i_X (svar_c "X") = false).
+Proof. reflexivity. Qed.
+Lemma test5: (strictly_positive (sp_not X_i_X_i_X)(svar_c "X") = false).
+Proof. reflexivity. Qed.
+Lemma test6: (strictly_positive X_i_X_i_nX (svar_c "X") = false).
+Proof. reflexivity. Qed.
+Lemma test7: (strictly_positive (sp_not X_i_X_i_nX) (svar_c "X") = true).
+Proof. reflexivity. Qed.
